examples/scache/AtomicIndexLookup.i.dfy
@@ -1,0 +1,52 @@
+include "Atomic.s.dfy"
+include "../../lib/Lang/NativeTypes.s.dfy"
+include "../../lib/Lang/LinearMaybe.s.dfy"
+include "CacheResources.i.dfy"
+include "Constants.i.dfy"
+
+module AtomicIndexLookupImpl {
+  import opened NativeTypes
+  import opened Ptrs
+  import opened AtomicSpec
+  import opened LinearMaybe
+  import opened NDiskPages
+
+  type AtomicIndexLookup = Atomic<uint64, CacheResources.R>
+
+  const NOT_MAPPED : uint64 := 0xffff_ffff_ffff_ffff;
+
+  predicate state_inv(v: uint64, g: CacheResources.R, disk_idx: int)
+  {
+    && (0 <= v as int < CacheSize() || v == NOT_MAPPED)
+    && g == CacheResources.DiskPageMap(disk_idx,
+        (if v == NOT_MAPPED then None else Some(v as int)))
+  }
+
+  predicate atomic_index_lookup_inv(a: AtomicStatus, ptr: Ptr)
+  {
+    forall v, g :: atomic_inv(a, v, g) <==> state_inv(v, g, ptr)
+  }
+
+  method atomic_index_lookup_read(
+      a: AtomicIndexLookup,
+      disk_idx: int)
+  returns (cache_idx: uint64)
+  requires atomic_index_lookup_inv(a, disk_idx)
+  ensures 0 <= cache_idx as int < CacheSize() || cache_idx == NOT_MAPPED
+
+  method atomic_index_lookup_add_mapping(
+      a: AtomicIndexLookup,
+      disk_idx: int,
+      cache_idx: int,
+      linear m: CacheResources.R)
+  returns (
+    success: bool,
+    linear m': CacheResources.R
+  )
+  requires m.CacheEntry?
+  requires m.disk_idx == None
+  requires m.cache_idx == cache_idx
+  ensures success ==> m' == m.(disk_idx := Some(disk_idx))
+  ensures success ==> m' == m.(disk_idx := Some(disk_idx))
+
+}
