examples/scache/CacheResources.i.dfy
@@ -1,0 +1,11 @@
+include "ResourceSpec.s.dfy"
+include "../../lib/Base/Multisets.i.dfy"
+include "../../lib/Base/Option.s.dfy"
+
+module CacheResource refines ResourceSpec {
+  import opened Options
+
+  datatype R =
+    | DiskPageMap(disk_idx: int, cache_idx: Option<int>)
+    | CacheEntry(disk_idx: Option<int>, cache_idx: int, data: seq<byte>)
+}
