examples/scache/Constants.i.dfy
@@ -1,0 +1,5 @@
+module Constants {
+  function method NThreads() : int { 24 }
+  function method CacheSize() : int { 1048576 }
+  function method NDiskPages() : int { 536870912 }
+}
